lib/Benchmarks/MPLSVectorizedProof.v
@@ -1,5 +1,84 @@
 Require Import Leapfrog.Benchmarks.ProofHeader.
-Require Import Leapfrog.Benchmarks.MPLSVectorized.
+Require Import Leapfrog.Benchmarks.MPLSVectorized. 
+
+Ltac compile_fm H el er :=
+  time "compilation correct" erewrite compilation_corr with (St1_eq_dec := el) (St2_eq_dec := er) in H.
+  
+  (* ;
+  simpl in H;
+  (* these could be invariants and somehow avoided completely
+      or if they have to be done it could all be done with reflection *)
+  time "antecedents" match goal with
+  | H0: _ <-> (?a -> ?b -> ?c -> ?d) |- _ =>
+    erewrite drop_antecedent_3 with (A := a) in H0;
+    [|
+      vm_compute; repeat econstructor |
+      vm_compute; repeat econstructor |
+      eapply in_In; exact eq_refl
+    ]
+
+  end;
+  crunch_foterm_ctx. *)
+
+Ltac decide_entailment H P HP el er P_orig e :=
+  let Horig := fresh "Horig" in
+  pose (P_orig := e);
+  time "remembering iff" remember_iff P HP e;
+  time "Horig" assert (Horig: P_orig <-> P)
+    by (rewrite HP; eapply iff_refl);
+  time "compile fm" compile_fm HP el er.
+
+(*   
+  match goal with
+  | HP: P <-> interp_fm ?v ?f |- _ =>
+      time "smt check neg" check_interp_neg (interp_fm v f);
+      idtac "UNSAT";
+      time "asserting neg" assert (~ P_orig) by (rewrite -> Horig; rewrite -> HP; apply dummy_pf_false)
+  | HP: P <-> interp_fm ?v ?f |- _ =>
+      time "smt check pos" check_interp_pos (interp_fm v f);
+      idtac "SAT";
+      time "asserting pos" assert (P_orig) by (rewrite -> Horig; rewrite -> HP; apply dummy_pf_true)
+  | |- _ => idtac "undecided goal :("
+  end;
+  time "clearing Horig" clear Horig. *)
+
+Ltac run_bisim_axiom el er use_hc :=
+  match goal with
+  | |- pre_bisimulation ?a ?r_states ?wp ?R (?C :: _) _ _ =>
+      let H := fresh "H" in
+      let P := fresh "P" in
+      let HP := fresh "HP" in
+      let P_orig := fresh "P_orig" in
+      decide_entailment H P HP el er P_orig (interp_entailment a
+                                                         (fun q1 q2 =>
+                                                            top' _ _ _ _ _ r_states
+                                                                 (conf_to_state_template q1)
+                                                                 (conf_to_state_template q2))
+                                                         ({| e_prem := R; e_concl := C |}))
+                                                         (* ;
+      match goal with
+      | HN: ~ P_orig |- _ =>
+          time "extending" (extend_bisim' HN use_hc; clear HN)
+      | H: P_orig |- pre_bisimulation _ _ _ _ (?C :: _) _ _ =>
+          time "skipping" (skip_bisim' H; clear H; try clear C)
+      end;
+      time "clearing all" clear P HP P_orig *)
+  end.
+
+Ltac solve_lang_equiv_state_axiom el er use_hc :=
+  eapply lang_equiv_to_pre_bisim;
+  time "init prebisim" (intros;
+  unfold mk_init;
+  erewrite Reachability.reachable_states_wit_conv; [
+    | repeat econstructor | econstructor; solve_fp_wit
+  ];
+  simpl);
+  time "build phase" run_bisim_axiom el er use_hc.
+  (* ;
+  time "close phase" close_bisim_axiom. *)
+
+
+  
 
 Lemma mpls_equiv:
   lang_equiv_state
